Meta.Test.Axiom.Extentionality

coq/ZF/Meta/Ctx.v
@@ -6,6 +6,8 @@ Import ListNotations.
 
 Definition Ctx : Type := list VarTy.
 
+Definition empty : Ctx := [].
+
 Fixpoint typeOf (G:Ctx) (n:nat) : option VarTy :=
   match G, n with
   | []        , _   => None
