coq/ZF/Meta/Sig.v
@@ -4,3 +4,5 @@ Require Import Coq.Strings.String.
 Require Import ZF.Meta.Ty.
 
 Definition Sig : Type := string -> option (list Ty * Ty).
+
+Definition empty : Sig := fun _ => None.
