coq/ZF/Meta/Test/Axiom/Extensionality.v
@@ -1,0 +1,24 @@
+Require Import ZF.Meta.Ctx.
+Require Import ZF.Meta.Sig.
+Require Import ZF.Meta.Term.
+Require Import ZF.Meta.Ty.
+
+(* Source: forall a b, (forall x, x :< a <-> x :< b) -> a = b.                  *)
+Definition Extensionality : Term :=
+  All VarTySet
+    (All VarTySet
+      (Imp
+        (All VarTySet
+          (Iff (Elem (Var 0) (Var 2))
+               (Elem (Var 0) (Var 1))))
+        (Equal (Var 1) (Var 0)))).
+
+(* The extensionality example is a proposition in the empty environment.        *)
+Proposition HasTy : HasTy Sig.empty Ctx.empty Extensionality TyProp.
+Proof.
+  apply HasTyAll, HasTyAll, HasTyImp.
+  - apply HasTyAll, HasTyIff.
+    + apply HasTyElem; apply (HasTyVar _ _ _ VarTySet); reflexivity.
+    + apply HasTyElem; apply (HasTyVar _ _ _ VarTySet); reflexivity.
+  - apply HasTyEqual;  apply (HasTyVar _ _ _ VarTySet); reflexivity.
+Qed.
